\documentclass{article}
\usepackage{epsfig}
\pagestyle{empty}
\begin{document}
$\text{cm}^2$
\pagebreak

\begin{equation} g = g_{max}n^4(E_0-V) \end{equation}
\pagebreak

$E_0$
\pagebreak

$n$
\pagebreak

\begin{equation} g = g_{max}q^2(E_0-V) \end{equation}
\pagebreak

$V$
\pagebreak

$q$
\pagebreak

\begin{equation} g = g_{max}m^3h(E_0-V) \end{equation}
\pagebreak

$m$
\pagebreak

$h$
\pagebreak

$\Omega.cm^2$
\pagebreak

\begin{equation} g = 10^6 . \frac{A}{\rho} \end{equation}
\pagebreak

$A$
\pagebreak

$\rho$
\pagebreak

$g$
\pagebreak

\begin{equation} \frac{dx(t)}{dt} = f(t, x(t)) \end{equation}
\pagebreak

\begin{align} k_1 &= f(t,x(t))\\ k_2 &= f(t+\frac{\Delta t}{2}, x(t) + \frac{\Delta t}{2}.k_1)\\ k_3 &= f(t+\frac{\Delta t}{2}, x(t) + \frac{\Delta t}{2}.k_2)\\ k_4 &= f(t+\Delta t, x(t) + \Delta t.k_3) \end{align}
\pagebreak

$\Delta t$
\pagebreak

$x(t+\Delta t)$
\pagebreak

\begin{equation} x(t+\Delta t) = x(t) + \frac{\Delta t}{6}(k_1 + 2k_2 + 2k_3+k_4) \end{equation}
\pagebreak

\begin{equation} g_c = \frac{2.10^2}{\frac{R_{cyt}l_1}{\pi r_1^2}+\frac{R_{cyt}l_2}{\pi r_2^2}} \end{equation}
\pagebreak

$g_c$
\pagebreak

$R_{cyt}$
\pagebreak

$l_1$
\pagebreak

$l_2$
\pagebreak

$r_1$
\pagebreak

$r_2$
\pagebreak

\begin{equation} GC = \left[\begin{array}{cccccccc} -g_c[0]&g_c[0]&0&...&...&0&0&0\\ g_c[0]&-g_c[0]-g_c[1]&g_c[1]&0&...&...&0&0\\ \vdots&&\ddots&&...&&0&0 \\ 0&...&g_c[i-1]&-g_c[i-1]-g_c[i]&g_c[i]&0&...&0\\ 0&0&0&...&...&&&0\\ 0&&...&&g_c[N-2]&-g_c[N-2]-g_c[N-1]&g_c[N-1]&0\\ 0&...&0&&&0&g_c[N-1]&-g_c[N-1]\end{array}\right] \end{equation}
\pagebreak

\begin{equation} a_{sat} = \frac{1-e^{-b.a_{nSat}}}{1+e^{-b.a_{nSat}}} \end{equation}
\pagebreak

\begin{equation} \resizebox{0.95\hsize}{!}{$Av(n) = \left[\begin{array}{ccccccccccc}a_1(n-1)&a_1(n-2)&e_1(n-1)&...&a_i(n-i)&a_i(n-2)&e_i(n-1)&...&a__{N_{MU}}(n-1)&a__{N_{MU}}(n-2)&e_{N_{MU}}(n-1)\end{array}\right]^T$} \end{equation}
\pagebreak

$a_i(n)$
\pagebreak

$i$
\pagebreak

$e_i(n)$
\pagebreak

$Av$
\pagebreak

\begin{equation} \resizebox{0.95\hsize}{!}{$\scriptstyle A = \left[\begin{array}{ccccccccccc}\scriptscriptstyle 2\exp\left(-\frac{T}{T_{c_1}}\right)&\scriptscriptstyle -\exp\left(-2\frac{T}{T_{c_1}}\right)&\scriptscriptstyle \frac{T^2}{T_{c_1}}\exp\left(1-\frac{T}{T_{c_1}} \right)&\scriptscriptstyle 0&\scriptscriptstyle ...&\scriptscriptstyle 0&\scriptscriptstyle 0& \scriptscriptstyle 0&\scriptscriptstyle 0&\scriptscriptstyle 0&\scriptscriptstyle 0\\ \scriptscriptstyle 0&\scriptscriptstyle 0&\scriptscriptstyle 0&\scriptscriptstyle \ddots&\scriptscriptstyle ...&&&&&\scriptscriptstyle ...&\scriptscriptstyle 0\\ \scriptscriptstyle 0&\scriptscriptstyle ...&&\scriptscriptstyle 0&\scriptscriptstyle 2\exp\left(-\frac{T}{T_{c_i}}\right)&\scriptscriptstyle -\exp\left(-2\frac{T}{T_{c_i}}\right)&\scriptscriptstyle \frac{T^2}{T_{c_i}}\exp\left(1-\frac{T}{T_{c_i}} \right)&\scriptscriptstyle 0&&&\scriptscriptstyle 0\\ \scriptscriptstyle0&\scriptscriptstyle0&\scriptscriptstyle...&&&\scriptscriptstyle0&\scriptscriptstyle 0&\scriptscriptstyle\ddots&\scriptscriptstyle0&\scriptscriptstyle0\\ \scriptscriptstyle0&\scriptscriptstyle0&\scriptscriptstyle0&\scriptscriptstyle...&&&&\scriptscriptstyle0&\scriptscriptstyle 2\exp\left(-\frac{T}{T_{c_{N_{MU}}}}\right)&\scriptscriptstyle -\exp\left(-2\frac{T}{T_{c_{N_{MU}}}}\right)&\scriptscriptstyle \frac{T^2}{T_{c_{{MU}}}}\exp\left(1-\frac{T}{T_{c_{N_{MU}}}} \right)\end{array}\right]$} \end{equation}
\pagebreak

$a$
\pagebreak

\begin{equation} a = A.Av \end{equation}
\pagebreak

$b$
\pagebreak

$1/T$
\pagebreak

\begin{equation} \Gamma = -\frac{1}{\lambda}\ln(\limits\prod_{i=1}^{\lambda} U(0,1)) \end{equation}
\pagebreak

$\lambda$
\pagebreak

$v$
\pagebreak

\begin{equation} v(t) = v_0\exp[-\beta(t-t_0)] \end{equation}
\pagebreak

$t_0$
\pagebreak

$v_0$
\pagebreak

\begin{equation} v(t) = 1 + (v_0 - 1)\exp[-\alpha(t-t_0)] \end{equation}
\pagebreak

\begin{equation} G = G_{max}(R_{on} + R_{off}) \end{equation}
\pagebreak

$G$
\pagebreak

$G_{max}$
\pagebreak

$N_{on}=\limits\sum_{i=1}g_{i_{on}}/G_{max}$
\pagebreak

$\tau_{on}=\frac{1}{\alpha.T_{max} +\beta}$
\pagebreak

\begin{equation} R_{on_{newValue}} = N_{on}r_{\infty}\Bigg[1-\exp\left(-\frac{t-t_0}{\tau_{on}}\right)\Bigg] + R_{on_{oldValue}}\exp\left(-\frac{t-t_0}{\tau_{on}}\right) \end{equation}
\pagebreak

\begin{equation} R_{off_{newValue}} = R_{off_{oldValue}}\exp\left(-\frac{t - t0}{\tau_{off}} \right) \end{equation}
\pagebreak

\begin{equation} r_{i_{newValue}} = r_{i_{oldValue}} \exp\left(\frac{t_i+T_{dur}-t}{\tau_{off}}\right) \end{equation}
\pagebreak

$\exp(T_{dur}/\tau_{on})$
\pagebreak

\begin{equation} r_{i_{newValue}} = r_{\infty} + (r_{i_{oldValue}} - r_{\infty}) \exp\left(\frac{T_{dur}}{\tau_{on}}\right) \end{equation}
\pagebreak

\begin{equation} R_{on_{newValue}} = R_{on_{oldValue}} + r_iS_{indCont} \end{equation}
\pagebreak

\begin{equation} R_{off_{newValue}} = R_{off_{oldValue}} - r_iS_{indCont} \end{equation}
\pagebreak

\begin{equation} R_{on_{newValue}} = R_{on_{oldValue}} - r_iS_{indCont} \end{equation}
\pagebreak

\begin{equation} R_{off_{newValue}} = R_{off_{oldValue}} + r_iS_{indCont} \end{equation}
\pagebreak

$G_{max} = \limits\sum_{i=1}^Ng_i$
\pagebreak

$\tau_{off}=\frac{1}{\beta}$
\pagebreak

\end{document}
